src/proof/create.v
@@ -8,92 +8,103 @@ Context `{!mapG Σ KKey.t PureKObject.t}.
 Context `{!mapG Σ KKey.t (gset KKey.t)}.
 Context `{!auth_setG Σ KKey.t}.
 
-Lemma wp_State__objCreate_pod_without_name γ l kind namespace obj
-  pod_ptr pod pure_pod parent_key owned_parent owned_child_keys:
+Lemma wp_State__objCreate_without_name γ l kind namespace obj
+  ptr kobj pure_kobj parent_key owned_parent owned_child_keys:
   {{{ is_pkg_init apimodel ∗
       "#Hisk" ∷ is_kubernetes γ l ∗
-      "%Hkind_is_pod" ∷ ⌜ kind = "Pod"%go ⌝ ∗
+      "%Hkind_eq" ∷ ⌜ kind = PureKObject.kind pure_kobj ⌝ ∗
       "%Hnamespace_is_parent_namespace" ∷ ⌜ namespace = parent_key.(KKey.Namespace') ⌝ ∗
       "%Hnamespace_valid" ∷ ⌜ namespace ≠ ""%go ∧ valid_namespace namespace ⌝ ∗
-      "%Hobj_is_pod" ∷ ⌜ obj = interface.mk (ptrT.id v1.Pod.id) #pod_ptr ⌝ ∗
-      "Hdeepown_l_pod" ∷ PurePod.deepown_l pod_ptr pod pure_pod 1 ∗
-      "%Hpure_pod_is_child" ∷ ⌜ obj_has_controller_parent_of (PureKObject.Pod pure_pod) parent_key.(KKey.Kind')
-        parent_key.(KKey.Name') (PureKObject.metadata owned_parent).(PureObjectMeta.UID') ⌝ ∗
-      "%Hwell_formed" ∷ ⌜ PurePod.well_formed_for_create_without_name pure_pod ⌝ ∗
+      "%Hinterface_agree" ∷ ⌜ PureKObject.interface_agree obj ptr pure_kobj ⌝ ∗
+      "Hdeepown_l" ∷ PureKObject.deepown_l ptr kobj pure_kobj 1 ∗
+      "%Hpure_kobj_is_child" ∷ ⌜ obj_has_controller_parent_of pure_kobj parent_key.(KKey.Kind')
+        parent_key.(KKey.Name') (PureKObject.objectmeta owned_parent).(PureObjectMeta.UID') ⌝ ∗
+      "%Hwell_formed" ∷ ⌜ PureKObject.well_formed_for_nameless_create pure_kobj ⌝ ∗
       "Hown_parent" ∷ parent_key [[ γ.(γ_state) ]]↦ owned_parent ∗
       "Hown_child_keys" ∷ parent_key [[ γ.(γ_children) ]]↦ owned_child_keys
   }}}
     l @ (ptrT.id apimodel.State.id) @ "objCreate" #kind #namespace #obj
-  {{{ created_pod_ptr created_pod created_pure_pod new_name new_key, RET (#(interface.mk (ptrT.id v1.Pod.id) #created_pod_ptr), #interface.nil);
-      "Hdeepown_created_pod" ∷ PurePod.deepown_l created_pod_ptr created_pod created_pure_pod 1 ∗
-      "%Hwell_formed" ∷ ⌜ PurePod.well_formed created_pure_pod ⌝ ∗
-      "%Hnamespace_matches" ∷ ⌜ created_pure_pod.(PurePod.ObjectMeta').(PureObjectMeta.Namespace') = namespace ⌝ ∗
-      "%Hname_matches" ∷ ⌜ created_pure_pod.(PurePod.ObjectMeta').(PureObjectMeta.Name') = new_name ⌝ ∗
-      "%Hnew_key_eq" ∷ ⌜ new_key = mk_pod_key namespace new_name ⌝ ∗
-      "%Hnew_key_notin" ∷ ⌜ new_key ∉ owned_child_keys ⌝ ∗
-      "Hown_created_pure_pod" ∷ new_key [[ γ.(γ_state) ]]↦ (PureKObject.Pod created_pure_pod) ∗
+  {{{ obj' ptr' kobj' pure_kobj', RET (#obj', #interface.nil);
+      "%Hinterface_agree'" ∷ ⌜ PureKObject.interface_agree obj' ptr' pure_kobj' ⌝ ∗
+      "%Hsame_cons" ∷ ⌜ PureKObject.same_constructor pure_kobj pure_kobj' ⌝ ∗
+      "Hdeepown_l'" ∷ PureKObject.deepown_l ptr' kobj' pure_kobj' 1 ∗
+      "%Hwell_formed" ∷ ⌜ PureKObject.well_formed pure_kobj' ⌝ ∗
+      "%Hnamespace_eq" ∷ ⌜ (PureKObject.objectmeta pure_kobj').(PureObjectMeta.Namespace') = namespace ⌝ ∗
+      "%Hnew_key_notin" ∷ ⌜ (PureKObject.key pure_kobj') ∉ owned_child_keys ⌝ ∗
+      "Hghost_pure_kobj'" ∷ (PureKObject.key pure_kobj') [[ γ.(γ_state) ]]↦ pure_kobj' ∗
       "Hown_parent" ∷ parent_key [[ γ.(γ_state) ]]↦ owned_parent ∗
-      "Hown_child_keys" ∷  parent_key [[ γ.(γ_children) ]]↦ (owned_child_keys ∪ {[new_key]}) ∗
-      "Hown_grandchild_keys" ∷ new_key [[ γ.(γ_children) ]]↦ ∅
-      (* TODO: specify that created_pod shares the same content with pod *)
+      "Hown_child_keys" ∷  parent_key [[ γ.(γ_children) ]]↦ (owned_child_keys ∪ {[PureKObject.key pure_kobj']}) ∗
+      "Hown_grandchild_keys" ∷ (PureKObject.key pure_kobj') [[ γ.(γ_children) ]]↦ ∅
+      (* TODO: specify that pure_kobj' shares some content with pure_kobj *)
   }}}.
 Proof.
   wp_start as "H". iNamed "H". iNamed "Hisk".
-  unfold PurePod.well_formed_for_create_without_name in Hwell_formed.
-  destruct Hwell_formed as (Hwell_formed_meta & Hwell_formed_spec & Hwell_formed_status).
-  unfold PureObjectMeta.well_formed_for_create_without_name in Hwell_formed_meta.
+  pose proof PureKObject.well_formed_for_nameless_create_split _ Hwell_formed as [Hwell_formed_meta Hwell_formed_other].
+  unfold PureObjectMeta.well_formed_for_nameless_create in Hwell_formed_meta.
   destruct Hwell_formed_meta as (Hgenerate_name & Hgenerate_name_len & Hname & Hnamespace & Howner_ref).
   destruct Hgenerate_name as (prefix & Hprefx & Hprefix_not_empty & Hvalid_prefix & Hnot_reserved_prefix).
   wp_apply wp_with_defer. iIntros (defer) "Hdefer". simpl subst. wp_auto.
   wp_apply wp_Mutex__Lock; [done|]. iIntros "[Hown_Mutex H]". iNamedPrefix "H" "Hinv_". wp_auto.
-  wp_apply (wp_deepCopy_pod with "[$Hdeepown_l_pod]"); [done|].
-  iIntros (copied_ptr copied_pod) "(Hdeepown_l_copied_pod & Hdeepown_l_pod)". wp_auto.
-  wp_apply wp_Accessor_pod; [done|]. rewrite bool_decide_true //. wp_auto.
-  iDestruct "Hdeepown_l_copied_pod" as "[Hcopied_ptr Hdeepown_copied_pod]".
-  iDestruct (struct_fields_split with "Hcopied_ptr") as "H". iNamed "H".
-  iNamedPrefix "Hdeepown_copied_pod" "Hcopied_pod_". iNamedPrefix "Hcopied_pod_Hdeepown_objectmeta" "Hcopied_pod_".
-  wp_apply (wp_SetNamespace with "[$HObjectMeta]"). iIntros "HObjectMeta". wp_auto.
-  wp_apply (wp_GetName with "[$HObjectMeta]"). iIntros "HObjectMeta". wp_auto.
-  wp_apply (wp_GetGenerateName with "[$HObjectMeta]"). iIntros "HObjectMeta". wp_auto.
-  assert (v1.ObjectMeta.Name' (v1.Pod.ObjectMeta' copied_pod) = ""%go) as -> by congruence.
-  wp_auto.
-  assert (v1.ObjectMeta.GenerateName' (v1.Pod.ObjectMeta' copied_pod) ≠ ""%go) as Hgenerate_name_not_empty.
-  { rewrite Hcopied_pod_Hdeepown_generatename. rewrite Hprefx. intro Hcontra. apply app_eq_nil in Hcontra.
+  wp_apply (wp_deepCopy with "[$Hdeepown_l]"); [done|].
+  iIntros (copied_i copied_ptr copied_kobj) "(%Hinterface_agree_copied & Hdeepown_l_copied & Hdeepown_l)". wp_auto.
+  wp_apply wp_Accessor; [done|]. rewrite bool_decide_true //. wp_auto.
+  iPoseProof (PureKObject.deepown_l_split _ _ _ _ with "Hdeepown_l_copied")
+    as "(Htypemeta_ptr & %Htypemeta_eq & Hdeepown_l_objectmeta & Hdeepown_l_other)".
+  iDestruct "Hdeepown_l_objectmeta" as "[Hobjectmeta_ptr Hdeepown_objectmeta]".
+  wp_apply (wp_SetNamespace with "[$Hobjectmeta_ptr]"). iIntros "Hobjectmeta_ptr". wp_auto.
+  wp_apply (wp_GetName with "[$Hobjectmeta_ptr]"). iIntros "Hobjectmeta_ptr". wp_auto.
+  wp_apply (wp_GetGenerateName with "[$Hobjectmeta_ptr]"). iIntros "Hobjectmeta_ptr". wp_auto.
+  iNamedPrefix "Hdeepown_objectmeta" "Hcopied_kobj_".
+  assert (v1.ObjectMeta.Name' (KObject.objectmeta copied_kobj) = ""%go) as -> by congruence. wp_auto.
+  assert (v1.ObjectMeta.GenerateName' (KObject.objectmeta copied_kobj) ≠ ""%go) as Hgenerate_name_not_empty.
+  { rewrite Hcopied_kobj_Hdeepown_generatename. rewrite Hprefx. intro Hcontra. apply app_eq_nil in Hcontra.
     destruct Hcontra as [_ Hcontra]. discriminate Hcontra. }
   wp_if_destruct; [done|]. rewrite bool_decide_false //. wp_auto.
-  assert (copied_pod.(v1.Pod.ObjectMeta').(v1.ObjectMeta.GenerateName') = prefix ++ "-"%go) as ->.
-  { rewrite Hcopied_pod_Hdeepown_generatename. intuition. }
+  assert (v1.ObjectMeta.GenerateName' (KObject.objectmeta copied_kobj) = prefix ++ "-"%go) as ->.
+  { rewrite Hcopied_kobj_Hdeepown_generatename. intuition. }
   wp_apply (wp_State__generateNewName _ _ _ _ _ (prefix ++ "-"%go) with "[$Hinv_Hstate_m_addr $Hinv_Hown_phys]").
   { eauto. }
   iIntros (new_name) "(%Hnew_name_valid & %Hnew_key_not_in_phys & %Hnew_name_not_reserved & Hinv_Hstate_m_addr & Hinv_Hown_phys)". wp_auto.
-  wp_apply (wp_SetName with "[$HObjectMeta]"). iIntros "HObjectMeta". wp_auto.
+  wp_apply (wp_SetName with "[$Hobjectmeta_ptr]"). iIntros "Hobjectmeta_ptr". wp_auto.
   wp_apply (wp_map_get with "[$Hinv_Hown_phys]"). iIntros "Hinv_Hown_phys". wp_auto.
   rewrite /is_Some Hnew_key_not_in_phys. wp_auto.
   wp_apply (wp_State__generateNewUIDAndUpdate with "[$Hinv_Hstate_used_uid_addr $Hinv_Hown_used_uid]").
   iIntros (generated_uid) "(%Hgenerated_uid_is_not_used & Hinv_Hstate_used_uid_addr & Hinv_Hown_used_uid)". wp_auto.
-  wp_apply (wp_SetUID with "[$HObjectMeta]"). iIntros "HObjectMeta". wp_auto.
+  wp_apply (wp_SetUID with "[$Hobjectmeta_ptr]"). iIntros "Hobjectmeta_ptr". wp_auto.
   wp_apply wp_strconv_FormatInt. iIntros (rv_str) "_". wp_auto.
-  wp_apply (wp_SetResourceVersion with "[$HObjectMeta]"). iIntros "HObjectMeta". wp_auto.
+  wp_apply (wp_SetResourceVersion with "[$Hobjectmeta_ptr]"). iIntros "Hobjectmeta_ptr". wp_auto.
   wp_apply (wp_map_insert with "[$Hinv_Hown_phys]"). iIntros "Hinv_Hown_phys". wp_auto.
-  iDestruct (struct_fields_combine (v:=v1.Pod.mk _ _ _ _)
-    with "[$HTypeMeta $HObjectMeta $HSpec $HStatus]") as "Hcopied_ptr". simpl.
-  iDestruct (rename_pod with "Hcopied_ptr") as (created_pod) "(Hcopied_ptr & %Hcreated_pod_eq)".
-  set created_pure_meta := pure_pod.(PurePod.ObjectMeta')
+  set new_objectmeta := KObject.objectmeta copied_kobj
+    <| v1.ObjectMeta.Namespace' := KKey.Namespace' parent_key |>
+    <| v1.ObjectMeta.Name' := new_name |>
+    <| v1.ObjectMeta.UID' := generated_uid |>
+    <| v1.ObjectMeta.ResourceVersion' := rv_str |>.
+  set new_pure_objectmeta := PureKObject.objectmeta pure_kobj
     <| PureObjectMeta.Namespace' := KKey.Namespace' parent_key |>
     <| PureObjectMeta.Name' := new_name |>
     <| PureObjectMeta.UID' := generated_uid |>
     <| PureObjectMeta.ResourceVersion' := rv_str |>.
-  set created_pure_pod := pure_pod <| PurePod.ObjectMeta' := created_pure_meta |>.
-  iCombineNamed "Hcopied_pod_*" as "H".
-  iAssert (PurePod.deepown created_pod created_pure_pod 1) with "[H]" as "Hdeepown_created_pod".
-  { iNamed "H". iFrame. iSplitR; [iPureIntro; rewrite Hcreated_pod_eq //|].
-    rewrite Hcreated_pod_eq //. iFrame. iPureIntro. done. }
-  wp_apply (wp_deepCopy_pod with "[Hcopied_ptr Hdeepown_created_pod]"); [iFrame;done|].
-  iIntros (returned_ptr returned_pod) "(Hdeepown_l_returned_pod & Hdeepown_l_created_pod)". wp_auto.
-  set new_key := {| KKey.Kind' := "Pod"; KKey.Name' := new_name; KKey.Namespace' := KKey.Namespace' parent_key |}.
+  iCombineNamed "Hcopied_kobj_*" as "H".
+  iAssert (PureObjectMeta.deepown_l (PureKObject.objectmeta_ptr copied_ptr pure_kobj) new_objectmeta new_pure_objectmeta 1)
+    with "[Hobjectmeta_ptr H]" as "Hdeepown_l_objectmeta".
+  { iNamed "H". iFrame. iPureIntro. done. }
+  iPoseProof (PureKObject.deepown_l_merge _ _ _ _ _ _ with "[Htypemeta_ptr Hdeepown_l_objectmeta Hdeepown_l_other]")
+    as "Hdeepown_l_copied".
+  { iFrame. done. }
+  wp_apply (wp_deepCopy with "[Hdeepown_l_copied]").
+  { iFrame. iPureIntro. destruct pure_kobj; exact Hinterface_agree_copied. }
+  iIntros (interface_obj' ptr' obj') "(%Hinterface_agree' & Hdeepown_l' & Hdeepown_l_copied)". wp_auto.
+  set new_key := {|
+    KKey.Kind' := PureKObject.kind pure_kobj;
+    KKey.Name' := new_name;
+    KKey.Namespace' := KKey.Namespace' parent_key
+  |}.
   fold new_key in Hnew_key_not_in_phys.
+  assert (new_key = PureKObject.key (PureKObject.update_objectmeta pure_kobj new_pure_objectmeta)) as Hnew_key_eq.
+  { unfold new_key. destruct pure_kobj; done. }
   iAssert (⌜ abs_state !! new_key = None ⌝%I) as "%Hnew_key_not_in_abs".
-  { iDestruct (big_sepM2_dom with "Hinv_Hphys_abs_rep") as %Hdom_eq. iPureIntro. apply not_elem_of_dom. apply not_elem_of_dom in Hnew_key_not_in_phys. set_solver. }
+  { iDestruct (big_sepM2_dom with "Hinv_Hphys_abs_rep") as %Hdom_eq. iPureIntro. apply not_elem_of_dom.
+    apply not_elem_of_dom in Hnew_key_not_in_phys. set_solver. }
   assert (children !! new_key = None) as Hnew_key_not_in_children.
   { destruct Hinv_Hghost_well_formed. apply not_elem_of_dom. apply not_elem_of_dom in Hnew_key_not_in_abs. set_solver. }
   iAssert (⌜ abs_state !! parent_key = Some (owned_parent) ⌝%I) as "%Hparent_key_in_abs".
@@ -110,54 +121,51 @@ Proof.
     { apply Hchildren_exist with (k := parent_key). exact Hparent_key_in_children. }
     apply not_elem_of_dom in Hnew_key_not_in_abs.
     set_solver. }
-  iMod (map_alloc new_key (PureKObject.Pod created_pure_pod) with "[$Hinv_Hown_abs]") as "[Hinv_Hown_abs Hown_pod]"; [eauto|].
+  iMod (map_alloc new_key (PureKObject.update_objectmeta pure_kobj new_pure_objectmeta) with "[$Hinv_Hown_abs]")
+    as "[Hinv_Hown_abs Hown_pod]"; [eauto|].
   iMod (auth_map.map_update _ _ (owned_child_keys ∪ {[new_key]}) with "Hinv_Hown_children Hown_child_keys")
     as "[Hinv_Hown_children Hown_child_keys]".
   iMod (map_alloc new_key ∅ with "[$Hinv_Hown_children]") as "[Hinv_Hown_children Hown_grandchild_keys]"; [eauto|].
-  set phys_state' := <[new_key:=interface.mk (ptrT.id v1.Pod.id) (# copied_ptr)]> phys_state.
+  set phys_state' := <[new_key:=copied_i]> phys_state.
   set used_uid' := <[generated_uid:=()]> used_uid.
-  set abs_state' := <[new_key:=PureKObject.Pod created_pure_pod]> abs_state.
+  set abs_state' := <[new_key:=PureKObject.update_objectmeta pure_kobj new_pure_objectmeta]> abs_state.
   set children' := (<[new_key:=∅]> (<[parent_key:=owned_child_keys ∪ {[new_key]}]> children)).
-  iAssert (state_rep phys_state' abs_state' %I) with "[Hdeepown_l_created_pod Hinv_Hphys_abs_rep]" as "Hinv_Hphys_abs_rep".
+  iAssert (state_rep phys_state' abs_state' %I) with "[Hdeepown_l_copied Hinv_Hphys_abs_rep]" as "Hinv_Hphys_abs_rep".
   { unfold state_rep. unfold phys_state'. unfold abs_state'.
     rewrite (big_sepM2_insert _ phys_state abs_state new_key _ _ Hnew_key_not_in_phys Hnew_key_not_in_abs).
-    iSplitL "Hdeepown_l_created_pod".
-    - unfold obj_rep.
-      assert (bool_decide (KKey.Kind' new_key = "Pod"%go) = true) as kind_is_pod.
-      { apply bool_decide_true. unfold new_key. simpl. reflexivity. }
-      rewrite kind_is_pod.
-      iExists copied_ptr, created_pod, created_pure_pod.
-      unfold pod_rep. iFrame "#". iFrame. iPureIntro. done.
+    iSplitL "Hdeepown_l_copied".
+    - iExists copied_ptr, (KObject.update_objectmeta copied_kobj new_objectmeta). iFrame. iPureIntro.
+      destruct pure_kobj; exact Hinterface_agree_copied.
     - done. }
-  assert (PurePod.well_formed created_pure_pod) as Hwell_formed.
-  { unfold PurePod.well_formed.
-    split_and!; [|intuition|intuition].
-    unfold PureObjectMeta.well_formed. 
-    split_and!.
-    1: intros; left; exists prefix; done.
-    all: intuition. }
+  assert (PureKObject.well_formed (PureKObject.update_objectmeta pure_kobj new_pure_objectmeta)) as Hwell_formed'.
+  { assert (PureObjectMeta.well_formed new_pure_objectmeta) as Hwell_formed_meta'.
+    { unfold PureObjectMeta.well_formed. 
+      split_and!.
+      1: intros; left; exists prefix; done. all: intuition. }
+    pose proof PureKObject.well_formed_implies _ Hwell_formed_other as Hwell_formed_other'.
+    apply PureKObject.well_formed_merge. split; [done|done]. }
   assert (ghost_well_formed (dom used_uid') abs_state' children' fresh_keys ) as Hinv_Hghost_well_formed'.
   {
-    assert (dom children' = dom children ∪ {[new_key]}) as Hdom_children_eq.
-    {
+    assert (dom children' = dom children ∪ {[new_key]}) as Hdom_children_eq. {
       unfold children'.
       rewrite !dom_insert_L.
       assert (parent_key ∈ dom children) as Hparent_in_dom.
       { apply elem_of_dom. exists owned_child_keys. exact Hparent_key_in_children. }
       assert ({[parent_key]} ∪ dom children = dom children) as ->.
       { set_solver. }
-      set_solver.
-    }
-    assert (PureObjectMeta.UID' (PureKObject.metadata (PureKObject.Pod created_pure_pod)) = generated_uid) as Hcreated_pure_pod_uiq_eq.
-    { intuition. }
+      set_solver. }
+    assert (PureObjectMeta.UID' (PureKObject.objectmeta (PureKObject.update_objectmeta pure_kobj new_pure_objectmeta)) = generated_uid)
+      as Hpure_pod'_uiq_eq.
+    { destruct pure_kobj; done. }
     assert (generated_uid ∉ dom used_uid) as Hgenerated_not_in_used.
     { apply not_elem_of_dom. exact Hgenerated_uid_is_not_used. }
-    assert (obj_has_controller_parent_of (PureKObject.Pod created_pure_pod) (KKey.Kind' parent_key)
-      (KKey.Name' parent_key) (PureObjectMeta.UID' (PureKObject.metadata owned_parent)))
-      as Hcreated_pure_pod_has_controller_parent_of_owned_parent by done.
+    assert (obj_has_controller_parent_of (PureKObject.update_objectmeta pure_kobj new_pure_objectmeta) (KKey.Kind' parent_key)
+      (KKey.Name' parent_key) (PureObjectMeta.UID' (PureKObject.objectmeta owned_parent)))
+      as Hpure_pod'_has_controller_parent_of_owned_parent.
+    { destruct pure_kobj; done. }
     destruct Hinv_Hghost_well_formed.
     apply mk_ghost_well_formed.
-    - intros k obj Hlookup. unfold abs_state' in Hlookup.
+    - intros k o Hlookup. unfold abs_state' in Hlookup.
       rewrite lookup_insert_Some in Hlookup.
       destruct Hlookup as [(<- & <-) | (Hk_neq & Hlookup)].
       + split; [done|done].
@@ -237,14 +245,14 @@ Proof.
       destruct Hlookup1 as [(<- & <-) | (Hk1_neq & Hlookup1)];
       destruct Hlookup2 as [(<- & <-) | (Hk2_neq & Hlookup2)].
       + done.
-      + assert ((PureKObject.metadata obj2).(PureObjectMeta.UID') ∈ dom used_uid) as Hobj2_uid_in_used.
+      + assert ((PureKObject.objectmeta obj2).(PureObjectMeta.UID') ∈ dom used_uid) as Hobj2_uid_in_used.
         { apply Hexisting_uid_is_used with (k := k2). done. }
-        rewrite <-Huid_eq, Hcreated_pure_pod_uiq_eq in Hobj2_uid_in_used. done.
-      + assert ((PureKObject.metadata obj1).(PureObjectMeta.UID') ∈ dom used_uid) as Hobj1_uid_in_used.
+        rewrite <-Huid_eq, Hpure_pod'_uiq_eq in Hobj2_uid_in_used. done.
+      + assert ((PureKObject.objectmeta obj1).(PureObjectMeta.UID') ∈ dom used_uid) as Hobj1_uid_in_used.
         { apply Hexisting_uid_is_used with (k := k1). done. }
-        rewrite Huid_eq Hcreated_pure_pod_uiq_eq in Hobj1_uid_in_used. done.
+        rewrite Huid_eq Hpure_pod'_uiq_eq in Hobj1_uid_in_used. done.
       + apply Hno_duplicate_uid with (obj1 := obj1) (obj2 := obj2); done.
-    - intros k obj Hlookup_abs_state. unfold abs_state', used_uid'.
+    - intros k o Hlookup_abs_state. unfold abs_state', used_uid'.
       rewrite dom_insert_L. rewrite lookup_insert_Some in Hlookup_abs_state.
       destruct Hlookup_abs_state as [(<- & <-) | (Hk_neq & Hlookup_abs_state)]; [set_solver|set_solver].
     - intros key_p obj_p key_c obj_c s Hlookup_p Hlookup_c Hlookup_children.
@@ -268,20 +276,21 @@ Proof.
           -- eapply Hchildren_point_to_parent; [done|done|done|done].
       + intros Hobj_has_controller_parent_of.
         destruct Hlookup_c as [(<- & <-) | (Hkey_c_neq & Hlookup_c)].
-        * assert (PureKObject.well_formed (PureKObject.Pod created_pure_pod)) as Hwell_formed_kobject by done.
-          pose proof (well_formed_obj_has_at_most_one_controller_parent (PureKObject.Pod created_pure_pod) Hwell_formed_kobject
-            _ _ _ _ _ _ Hobj_has_controller_parent_of Hcreated_pure_pod_has_controller_parent_of_owned_parent) as (Hkind_eq & Hname_eq & Huid_eq).
+        * pose proof (well_formed_obj_has_at_most_one_controller_parent
+            (PureKObject.update_objectmeta pure_kobj new_pure_objectmeta) Hwell_formed' _ _ _ _ _ _
+            Hobj_has_controller_parent_of Hpure_pod'_has_controller_parent_of_owned_parent)
+            as (Hkind_eq & Hname_eq & Huid_eq).
           destruct Hlookup_p as [(<- & <-) | (Hkey_p_neq & Hlookup_p)].
           -- exfalso.
             pose proof (Hexisting_uid_is_used parent_key owned_parent Hparent_key_in_abs).
-            rewrite Hcreated_pure_pod_uiq_eq in Huid_eq.
+            rewrite Hpure_pod'_uiq_eq in Huid_eq.
             rewrite <-Huid_eq in H. done.
           -- pose proof (Hno_duplicate_uid _ _ _ _ Hlookup_p Hparent_key_in_abs Huid_eq) as ->.
             destruct Hlookup_children as [(Hkey_p_eq_new & <-) | (Hkey_p_neq' & Hlookup_children)]; [done|].
             rewrite lookup_insert_Some in Hlookup_children.
             destruct Hlookup_children as [(Hkey_p_eq_new & <-) | (Hkey_p_neq'' & Hlookup_children)]; [set_solver|done].
         * destruct Hlookup_p as [(<- & <-) | (Hkey_p_neq & Hlookup_p)].
-          -- rewrite Hcreated_pure_pod_uiq_eq in Hobj_has_controller_parent_of.
+          -- rewrite Hpure_pod'_uiq_eq in Hobj_has_controller_parent_of.
             pose proof (Hparent_uid_is_used _ _ _ _ _ Hlookup_c Hobj_has_controller_parent_of).
             done.
           -- destruct Hlookup_children as [(Hkey_p_eq_new & <-) | (Hkey_p_neq' & Hlookup_children)]; [done|].
@@ -290,66 +299,71 @@ Proof.
             ++ rewrite Hparent_key_in_abs in Hlookup_p. injection Hlookup_p as <-.
               pose proof ((proj2 (Hchildren_point_to_parent _ _ _ _ _ Hparent_key_in_abs Hlookup_c Hparent_key_in_children))).
               set_solver.
-            ++ pose proof ((proj2 (Hchildren_point_to_parent _ _ _ _ _ Hlookup_p Hlookup_c Hlookup_children)) Hobj_has_controller_parent_of).
+            ++ pose proof ((proj2 (Hchildren_point_to_parent _ _ _ _ _ Hlookup_p Hlookup_c Hlookup_children))
+                Hobj_has_controller_parent_of).
               done.
-    - intros k obj kind name uid Hlookup_abs Hhas_parent.
+    - intros k o kind name uid Hlookup_abs Hhas_parent.
       unfold abs_state' in Hlookup_abs.
       rewrite lookup_insert_Some in Hlookup_abs.
       destruct Hlookup_abs as [(<- & <-) | (Hk_neq & Hlookup_abs)].
-      + assert (PureKObject.well_formed (PureKObject.Pod created_pure_pod)) as Hwell_formed_kobject by done.
-        pose proof (well_formed_obj_has_at_most_one_controller_parent (PureKObject.Pod created_pure_pod) Hwell_formed_kobject
-          _ _ _ _ _ _ Hhas_parent Hcreated_pure_pod_has_controller_parent_of_owned_parent) as (Hkind_eq & Hname_eq & ->).
+      + pose proof (well_formed_obj_has_at_most_one_controller_parent
+          (PureKObject.update_objectmeta pure_kobj new_pure_objectmeta) Hwell_formed' _ _ _ _ _ _ Hhas_parent
+          Hpure_pod'_has_controller_parent_of_owned_parent) as (Hkind_eq & Hname_eq & ->).
         pose proof (Hexisting_uid_is_used parent_key owned_parent Hparent_key_in_abs).
         unfold used_uid'. set_solver.
-      + pose proof (Hparent_uid_is_used k obj kind name uid Hlookup_abs Hhas_parent).
+      + pose proof (Hparent_uid_is_used k o kind name uid Hlookup_abs Hhas_parent).
         unfold used_uid'. set_solver.
   }
   iCombineNamed "Hinv_*" as "H".
   wp_apply (wp_Mutex__Unlock _ (kubernetes_inv γ l) with "[$Hown_Mutex H]").
   { iNamed "H". iFrame. iFrame "#". done. }
-  iApply "HΦ". iFrame "Hdeepown_l_returned_pod". iFrame. done.
+  iApply "HΦ". iFrame "Hdeepown_l'". iFrame. rewrite <-Hnew_key_eq. iFrame. iPureIntro. split_and!.
+  all: try done; destruct pure_kobj; done.
 Qed.
 
-Lemma wp_State__PodCreate_without_name γ l namespace pod_ptr
+Lemma wp_State__PodCreate_without_name γ l namespace ptr
   pod pure_pod parent_key owned_parent owned_child_keys:
   {{{ is_pkg_init apimodel ∗
       "#Hisk" ∷ is_kubernetes γ l ∗
       "%Hnamespace_is_parent_namespace" ∷ ⌜ namespace = parent_key.(KKey.Namespace') ⌝ ∗
       "%Hnamespace_valid" ∷ ⌜ namespace ≠ ""%go ∧ valid_namespace namespace ⌝ ∗
-      "Hdeepown_l_pod" ∷ PurePod.deepown_l pod_ptr pod pure_pod 1 ∗
+      "Hdeepown_l" ∷ PurePod.deepown_l ptr pod pure_pod 1 ∗
       "%Hpure_pod_is_child" ∷ ⌜ obj_has_controller_parent_of (PureKObject.Pod pure_pod) parent_key.(KKey.Kind')
-        parent_key.(KKey.Name') (PureKObject.metadata owned_parent).(PureObjectMeta.UID') ⌝ ∗
-      "#Hwell_formed" ∷ ⌜ PurePod.well_formed_for_create_without_name pure_pod ⌝ ∗
+        parent_key.(KKey.Name') (PureKObject.objectmeta owned_parent).(PureObjectMeta.UID') ⌝ ∗
+      "#Hwell_formed" ∷ ⌜ PurePod.well_formed_for_nameless_create pure_pod ⌝ ∗
       "Hown_parent" ∷ parent_key [[ γ.(γ_state) ]]↦ owned_parent ∗
       "Hown_child_keys" ∷ parent_key [[ γ.(γ_children) ]]↦ owned_child_keys
   }}}
-    l @ (ptrT.id apimodel.State.id) @ "PodCreate" #namespace #pod_ptr
-  {{{ created_pod_ptr created_pod created_pure_pod new_name new_key, RET (#created_pod_ptr, #interface.nil);
-      "Hdeepown_created_pod" ∷ PurePod.deepown_l created_pod_ptr created_pod created_pure_pod 1 ∗
-      "%Hwell_formed" ∷ ⌜ PurePod.well_formed created_pure_pod ⌝ ∗
-      "%Hnamespace_matches" ∷ ⌜ created_pure_pod.(PurePod.ObjectMeta').(PureObjectMeta.Namespace') = namespace ⌝ ∗
-      "%Hname_matches" ∷ ⌜ created_pure_pod.(PurePod.ObjectMeta').(PureObjectMeta.Name') = new_name ⌝ ∗
-      "%Hnew_key_eq" ∷ ⌜ new_key = mk_pod_key namespace new_name ⌝ ∗
-      "%Hnew_key_notin" ∷ ⌜ new_key ∉ owned_child_keys ⌝ ∗
-      "Hown_created_pure_pod" ∷ new_key [[ γ.(γ_state) ]]↦ (PureKObject.Pod created_pure_pod) ∗
+    l @ (ptrT.id apimodel.State.id) @ "PodCreate" #namespace #ptr
+  {{{ ptr' pod' pure_pod', RET (#ptr', #interface.nil);
+      "Hdeepown_pod'" ∷ PurePod.deepown_l ptr' pod' pure_pod' 1 ∗
+      "%Hwell_formed" ∷ ⌜ PurePod.well_formed pure_pod' ⌝ ∗
+      "%Hnamespace_matches" ∷ ⌜ pure_pod'.(PurePod.ObjectMeta').(PureObjectMeta.Namespace') = namespace ⌝ ∗
+      "%Hnew_key_notin" ∷ ⌜ (PurePod.key pure_pod') ∉ owned_child_keys ⌝ ∗
+      "Hown_pure_pod'" ∷ (PurePod.key pure_pod') [[ γ.(γ_state) ]]↦ (PureKObject.Pod pure_pod') ∗
       "Hown_parent" ∷ parent_key [[ γ.(γ_state) ]]↦ owned_parent ∗
-      "Hown_child_keys" ∷  parent_key [[ γ.(γ_children) ]]↦ (owned_child_keys ∪ {[new_key]}) ∗
-      "Hown_grandchild_keys" ∷ new_key [[ γ.(γ_children) ]]↦ ∅
-      (* TODO: specify that created_pod shares some contents with pod *)
+      "Hown_child_keys" ∷  parent_key [[ γ.(γ_children) ]]↦ (owned_child_keys ∪ {[PurePod.key pure_pod']}) ∗
+      "Hown_grandchild_keys" ∷ (PurePod.key pure_pod') [[ γ.(γ_children) ]]↦ ∅
+      (* TODO: specify that pod' shares some contents with pod *)
   }}}.
 Proof.
-  wp_start as "H". iNamed "H". iNamed "Hisk". wp_auto. wp_alloc pod_ptr_ptr as "Hpod_ptr_ptr". wp_auto.
-  wp_apply (wp_State__objCreate_pod_without_name with "[$Hdeepown_l_pod $Hown_child_keys $Hown_parent]").
+  wp_start as "H". iNamed "H". iNamed "Hisk". wp_auto.
+  wp_apply (wp_State__objCreate_without_name _ _ _ _ _ _ (KObject.Pod pod) (PureKObject.Pod pure_pod)
+  with "[$Hdeepown_l $Hown_child_keys $Hown_parent]").
   { iFrame "#". done. }
-  iIntros (created_pod_ptr created_pod created_pure_pod new_name new_key) "H". iNamed "H". wp_auto.
+  iIntros (obj' ptr' kobj' pure_kobj') "H". iNamed "H". wp_auto.
+  assert (∃ pure_pod', pure_kobj' = PureKObject.Pod pure_pod') as [pure_pod' ->].
+  { destruct pure_kobj'; try done. exists p. done. }
+  iPoseProof (PureKObject.pod_deepown_l with "Hdeepown_l'") as "(%pod' & -> & Hdeepown_l')".
   rewrite bool_decide_true //. wp_auto.
+  unfold PureKObject.interface_agree in Hinterface_agree'. rewrite Hinterface_agree'.
   unshelve wp_apply wp_interface_checked_type_assert; try tc_solve.
-  { iPureIntro. intros ptr_id. exists created_pod_ptr. done. }
+  { iPureIntro. intros ptr_id. exists ptr'. done. }
   iIntros (y ok) "%if_ok".
   assert (ok = true) as ->.
   { destruct ok; [done|]. intuition. }
   wp_auto.
-  assert (created_pod_ptr = y) as ->.
+  assert (ptr' = y) as ->.
   { inversion if_ok. apply (inj to_val). done. }
   iApply "HΦ". iFrame. done.
 Qed.
