src/proof/delete.v
@@ -8,21 +8,21 @@ Context `{!mapG Σ KKey.t PureKObject.t}.
 Context `{!mapG Σ KKey.t (gset KKey.t)}.
 Context `{!auth_setG Σ KKey.t}.
 
-Lemma wp_State__objDelete_pod γ l key
-  pure_pod parent_key owned_child_keys owned_grandchild_keys:
+Lemma wp_State__objDelete γ l key
+  pure_kobj parent_key owned_child_keys owned_grandchild_keys:
   {{{ is_pkg_init apimodel ∗
       "#Hisk" ∷ is_kubernetes γ l ∗
-      "%Hpod_is_child" ∷ ⌜ key ∈ owned_child_keys ⌝ ∗
-      "%Hkind_is_pod" ∷ ⌜ KKey.Kind' key = "Pod"%go ⌝ ∗
-      "Hown_pod" ∷ key [[ γ.(γ_state) ]]↦ (PureKObject.Pod pure_pod) ∗
+      "%Hkind_eq" ∷ ⌜ KKey.Kind' key = PureKObject.kind pure_kobj ⌝ ∗
+      "%His_child" ∷ ⌜ key ∈ owned_child_keys ⌝ ∗
+      "Hghost_pure_kobj" ∷ key [[ γ.(γ_state) ]]↦ pure_kobj ∗
       "Hown_child_keys" ∷ parent_key [[ γ.(γ_children) ]]↦ owned_child_keys ∗
       "Hown_grandchild_keys" ∷ key [[ γ.(γ_children) ]]↦ owned_grandchild_keys
   }}}
     l @ (ptrT.id apimodel.State.id) @ "objDelete" #key
-  {{{ updated_pure_pod, RET #interface.nil;
-      "Hpod_updated_or_deleted" ∷ ((
-        "%Hts" ∷ ⌜ updated_pure_pod.(PurePod.ObjectMeta').(PureObjectMeta.DeletionTimestamp') ≠ None ⌝ ∗
-        "Hown_pod" ∷ key [[ γ.(γ_state) ]]↦ (PureKObject.Pod updated_pure_pod) ∗
+  {{{ (pure_kobj': PureKObject.t), RET #interface.nil;
+      (("%Hsame_cons" ∷ ⌜ PureKObject.same_constructor pure_kobj pure_kobj' ⌝ ∗
+        "%Hts" ∷ ⌜ (PureKObject.objectmeta pure_kobj').(PureObjectMeta.DeletionTimestamp') ≠ None ⌝ ∗
+        "Hghost_pure_kobj" ∷ key [[ γ.(γ_state) ]]↦ pure_kobj' ∗
         "Hown_child_keys" ∷ parent_key [[ γ.(γ_children) ]]↦ owned_child_keys ∗
         "Hown_grandchild_keys" ∷ key [[ γ.(γ_children) ]]↦ owned_grandchild_keys
       ) ∨
@@ -31,90 +31,82 @@ Lemma wp_State__objDelete_pod γ l key
 Proof.
   wp_start as "H". iNamed "H". iNamed "Hisk". wp_apply wp_with_defer. iIntros (defer) "Hdefer". simpl subst. wp_auto.
   wp_apply wp_Mutex__Lock; [done|]. iIntros "[Hown_Mutex H]". iNamedPrefix "H" "Hinv_". wp_auto.
-  iAssert (⌜ abs_state !! key = Some (PureKObject.Pod pure_pod) ⌝%I) as "%Hkey_in_abs".
-  { iDestruct (map_valid with "Hinv_Hown_abs Hown_pod") as %Hlookup. iPureIntro; done. }
+  iAssert (⌜ abs_state !! key = Some pure_kobj ⌝%I) as "%Hkey_in_abs".
+  { iDestruct (map_valid with "Hinv_Hown_abs Hghost_pure_kobj") as %Hlookup. iPureIntro; done. }
   iAssert (⌜ children !! parent_key = Some owned_child_keys ⌝%I) as "%Hparent_key_in_children".
   { iDestruct (map_valid with "Hinv_Hown_children Hown_child_keys") as %Hlookup. iPureIntro; done. }
   iAssert (⌜ children !! key = Some owned_grandchild_keys ⌝%I) as "%Hkey_in_children".
   { iDestruct (map_valid with "Hinv_Hown_children Hown_grandchild_keys") as %Hlookup. iPureIntro; done. }
-  iAssert (⌜ ∃ obj, phys_state !! key = Some obj ⌝%I) as "%Hkey_in_phys".
-  {
+  iAssert (⌜ ∃ obj, phys_state !! key = Some obj ⌝%I) as "%Hkey_in_phys". {
     iDestruct (big_sepM2_lookup_r with "Hinv_Hphys_abs_rep") as (obj Hkey_in_phys) "_"; [done|].
-    iPureIntro. exists obj. done.
-  }
+    iPureIntro. exists obj. done. }
   destruct Hkey_in_phys as [obj Hkey_in_phys].
   iDestruct (big_sepM2_delete _ phys_state abs_state key _ _ Hkey_in_phys Hkey_in_abs
     with "Hinv_Hphys_abs_rep") as "[Hk_rep Hother_rep]".
-  destruct decide_kind_is_pod with (KKey.Kind' key) as [kind_is_pod kind_is_not_replicaset]; [done|].
-  iAssert (∃ ptr pod pure_pod', pod_rep obj (PureKObject.Pod pure_pod) ptr pod pure_pod')%I
-  with "[Hk_rep]" as "(%ptr & %pod & %pure_pod' & Hpod_rep)".
-  { unfold obj_rep. rewrite kind_is_pod. iDestruct "Hk_rep" as "(%ptr & %pod & %pure_pod' & H)". iExists ptr, pod, pure_pod'. iFrame. }
-  iNamed "Hpod_rep".
-  injection Habs_v_is_pod as <-.
+  iDestruct "Hk_rep" as "(%ptr & %kobj & %Hinterface_agree & Hdeepown_l)".
   wp_apply (wp_map_get with "[$Hinv_Hown_phys]"). iIntros "Hinv_Hown_phys". wp_auto.
-  rewrite /is_Some Hkey_in_phys. wp_auto.
-  wp_apply wp_Accessor_pod; [done|].
-  assert ((bool_decide (interface.nil = interface.nil)) = true) as nil_is_nil.
-  { rewrite bool_decide_true //. }
-  rewrite nil_is_nil. wp_auto.
-  iDestruct "Hdeepown_l_pod" as "[Hpod_ptr Hdeepown_pod]".
-  iDestruct (struct_fields_split with "Hpod_ptr") as "H". iNamed "H".
-  wp_apply (wp_GetFinalizers with "[$HObjectMeta]").
-  iIntros "HObjectMeta". wp_auto.
+  rewrite /is_Some Hkey_in_phys bool_decide_true //; [exists obj; done|]. wp_auto.
+  wp_apply wp_Accessor; [done|]. rewrite bool_decide_true //. wp_auto.
+  iPoseProof (PureKObject.deepown_l_split _ _ _ _ with "Hdeepown_l")
+    as "(Htypemeta_ptr & %Htypemeta_eq & Hdeepown_l_objectmeta & Hdeepown_l_other)".
+  iDestruct "Hdeepown_l_objectmeta" as "[Hobjectmeta_ptr Hdeepown_objectmeta]".
+  wp_apply (wp_GetFinalizers with "[$Hobjectmeta_ptr]"). iIntros "Hobjectmeta_ptr". wp_auto.
   wp_if_destruct.
-  - wp_apply (wp_GetDeletionTimestamp with "[$HObjectMeta]"). iIntros "HObjectMeta". wp_auto.
+  - wp_apply (wp_GetDeletionTimestamp with "[$Hobjectmeta_ptr]"). iIntros "Hobjectmeta_ptr". wp_auto.
     wp_if_destruct.
     + wp_apply v1.wp_Now. iIntros (time pure_time) "Hdeepown_time". wp_auto.
-      wp_apply (wp_SetDeletionTimestamp with "[$HObjectMeta]"). iIntros "HObjectMeta". wp_auto.
+      wp_apply (wp_SetDeletionTimestamp with "[$Hobjectmeta_ptr]"). iIntros "Hobjectmeta_ptr". wp_auto.
       wp_apply wp_strconv_FormatInt. iIntros (rv_str) "_". wp_auto.
-      wp_apply (wp_SetResourceVersion with "[$HObjectMeta]"). iIntros "HObjectMeta". wp_auto.
-      iDestruct (struct_fields_combine (v:=v1.Pod.mk _ _ _ _)
-        with "[$HTypeMeta $HObjectMeta $HSpec $HStatus]") as "Hpod_ptr". simpl.
-      iDestruct (rename_pod with "Hpod_ptr") as "(%updated_pod & Hpod_ptr & %Hupdated_pod_eq)".
-      set updated_pure_meta := pure_pod.(PurePod.ObjectMeta')
-        <| PureObjectMeta.ResourceVersion' := rv_str |>
-        <| PureObjectMeta.DeletionTimestamp' := Some pure_time |>.
-      set updated_pure_pod := pure_pod <| PurePod.ObjectMeta' := updated_pure_meta |>.
-      iMod (auth_map.map_update _ _ (PureKObject.Pod updated_pure_pod) with "Hinv_Hown_abs Hown_pod")
-        as "[Hinv_Hown_abs Hown_pod]".
-      iAssert (state_rep phys_state (<[key:=PureKObject.Pod updated_pure_pod]> abs_state) %I)
-      with "[Hpod_ptr Hdeepown_pod Hother_rep Hdeepown_time now]" as "Hinv_Hphys_abs_rep".
-      { assert (delete key abs_state = delete key (<[key:=PureKObject.Pod updated_pure_pod]> abs_state)) as ->.
-        { rewrite delete_insert_eq. reflexivity. }
-        iApply (big_sepM2_delete _ phys_state (<[key:=PureKObject.Pod updated_pure_pod]> abs_state) key _ (PureKObject.Pod updated_pure_pod)
-          Hkey_in_phys with "[$Hother_rep Hpod_ptr Hdeepown_pod Hdeepown_time now]").
-        { rewrite lookup_insert. destruct (decide (key = key)) as [|Hcontra]; [done|done]. }
-        unfold obj_rep. rewrite kind_is_pod. iExists ptr, updated_pod, updated_pure_pod. unfold pod_rep.
-        iSplit;[done|iSplit;[done|]].
-        iNamed "Hdeepown_pod". iFrame. iSplitR; [iPureIntro; rewrite Hupdated_pod_eq //|].
-        iNamed "Hdeepown_objectmeta". rewrite Hupdated_pod_eq //.
-        iAssert (⌜ now_ptr ≠ null ⌝%I) as "%now_ptr_not_null".
+      wp_apply (wp_SetResourceVersion with "[$Hobjectmeta_ptr]"). iIntros "Hobjectmeta_ptr". wp_auto.
+      set new_pure_objectmeta := PureKObject.objectmeta pure_kobj
+        <| PureObjectMeta.DeletionTimestamp' := Some pure_time |>
+        <| PureObjectMeta.ResourceVersion' := rv_str |>.
+      set new_objectmeta := KObject.objectmeta kobj
+        <| v1.ObjectMeta.DeletionTimestamp' := now_ptr |>
+        <| v1.ObjectMeta.ResourceVersion' := rv_str |>.
+      iAssert (PureObjectMeta.deepown_l (PureKObject.objectmeta_ptr ptr pure_kobj) new_objectmeta new_pure_objectmeta 1)
+        with "[Hobjectmeta_ptr Hdeepown_objectmeta now Hdeepown_time]" as "Hdeepown_l_objectmeta".
+      { iAssert (⌜ now_ptr ≠ null ⌝%I) as "%now_ptr_not_null".
         { by iDestruct (typed_pointsto_not_null with "now") as %?. }
-        iFrame. iPureIntro. done. }
-      assert (ghost_well_formed (dom used_uid) (<[key:=PureKObject.Pod updated_pure_pod]> abs_state) children fresh_keys)
-      as Hinv_Hghost_well_formed'.
+        iNamed "Hdeepown_objectmeta". iFrame. iPureIntro. split_and!; done. }
+      iPoseProof (PureKObject.deepown_l_merge _ _ _ _ _ _ with "[Htypemeta_ptr Hdeepown_l_objectmeta Hdeepown_l_other]")
+        as "Hdeepown_l".
+      { iFrame. done. }
+      set updated_kobj := (KObject.update_objectmeta kobj new_objectmeta).
+      set updated_pure_kobj := (PureKObject.update_objectmeta pure_kobj new_pure_objectmeta).
+      iMod (auth_map.map_update _ _ updated_pure_kobj with "Hinv_Hown_abs Hghost_pure_kobj")
+        as "[Hinv_Hown_abs Hghost_pure_kobj]".
+      iAssert (state_rep phys_state (<[key:=updated_pure_kobj]> abs_state) %I)
+        with "[Hdeepown_l Hother_rep]" as "Hinv_Hphys_abs_rep".
+      { assert (delete key abs_state = delete key (<[key:=updated_pure_kobj]> abs_state)) as ->.
+        { rewrite delete_insert_eq. reflexivity. }
+        iApply (big_sepM2_delete _ phys_state (<[key:=updated_pure_kobj]> abs_state) key _ (updated_pure_kobj)
+          Hkey_in_phys with "[$Hother_rep Hdeepown_l]").
+        { rewrite lookup_insert. destruct (decide (key = key)) as [|Hcontra]; [done|done]. }
+        iExists ptr, updated_kobj. iFrame. iPureIntro. destruct pure_kobj; done. }
+      assert (ghost_well_formed (dom used_uid) (<[key:=updated_pure_kobj]> abs_state) children fresh_keys)
+        as Hinv_Hghost_well_formed'.
       {
         destruct Hinv_Hghost_well_formed.
         assert (parent_key ≠ key) as parent_neq_key.
-        { specialize (Hno_self_parenting parent_key owned_child_keys key Hparent_key_in_children Hpod_is_child). done. }
-        assert (dom (<[key:=PureKObject.Pod updated_pure_pod]> abs_state) = dom abs_state) as abs_dom_simpl.
+        { specialize (Hno_self_parenting parent_key owned_child_keys key Hparent_key_in_children His_child). done. }
+        assert (dom (<[key:=updated_pure_kobj]> abs_state) = dom abs_state) as abs_dom_simpl.
         { rewrite dom_insert_L.
           assert ({[key]} ∪ dom abs_state = dom abs_state) as ->.
           { set_solver. }
           reflexivity. }
-        assert ((PureKObject.metadata (PureKObject.Pod updated_pure_pod)).(PureObjectMeta.OwnerReferences') = (PureKObject.metadata (PureKObject.Pod pure_pod)).(PureObjectMeta.OwnerReferences'))
-        as updated_pure_pod_owner_references_eq.
-        { simpl. subst updated_pure_pod. simpl. reflexivity. }
-        assert ((PureKObject.metadata (PureKObject.Pod updated_pure_pod)).(PureObjectMeta.UID') = (PureKObject.metadata (PureKObject.Pod pure_pod)).(PureObjectMeta.UID'))
-        as updated_pure_pod_uid_eq.
-        { simpl. subst updated_pure_pod. simpl. reflexivity. }
-        assert (key = PureKObject.key (PureKObject.Pod updated_pure_pod) ∧ PureKObject.well_formed (PureKObject.Pod updated_pure_pod))
+        assert ((PureKObject.objectmeta updated_pure_kobj).(PureObjectMeta.OwnerReferences') = (PureKObject.objectmeta pure_kobj).(PureObjectMeta.OwnerReferences'))
+        as updated_pure_kobj_owner_references_eq.
+        { destruct pure_kobj; done. }
+        assert ((PureKObject.objectmeta updated_pure_kobj).(PureObjectMeta.UID') = (PureKObject.objectmeta pure_kobj).(PureObjectMeta.UID'))
+        as updated_pure_kobj_uid_eq.
+        { destruct pure_kobj; done. }
+        assert (key = PureKObject.key updated_pure_kobj ∧ PureKObject.well_formed updated_pure_kobj)
           as [Hagree Hwell_formed].
-        { assert (key = PureKObject.key (PureKObject.Pod pure_pod) ∧ PureKObject.well_formed (PureKObject.Pod pure_pod))
-          as [Hagree Hwell_formed].
-          { apply Habs_state_well_formed. done. } done. }
+        { assert (key = PureKObject.key pure_kobj ∧ PureKObject.well_formed pure_kobj) as [Hagree Hwell_formed].
+          { apply Habs_state_well_formed. done. } destruct pure_kobj; done. }
         apply mk_ghost_well_formed.
-        - intros k obj Hlookup.
+        - intros k o Hlookup.
           rewrite lookup_insert_Some in Hlookup.
           destruct Hlookup as [(<- & <-) | (Hk_neq & Hlookup)].
           + done.
@@ -137,10 +129,10 @@ Proof.
           + eapply Hno_duplicate_uid; [eauto|eauto|].
             rewrite Huid_eq -Hobj2_eq. done.
           + eapply Hno_duplicate_uid; [eauto|eauto|done].
-        - intros k obj Hlookup.
+        - intros k o Hlookup.
           rewrite lookup_insert_Some in Hlookup.
           destruct Hlookup as [(<- & <-) | (Hk_neq & Hlookup_obj)].
-          + rewrite updated_pure_pod_uid_eq. eapply Hexisting_uid_is_used. done.
+          + rewrite updated_pure_kobj_uid_eq. eapply Hexisting_uid_is_used. done.
           + eapply Hexisting_uid_is_used. done.
         - intros key_p obj_p key_c obj_c s Hlookup_p Hlookup_c Hlookup_children.
           rewrite lookup_insert_Some in Hlookup_p.
@@ -149,44 +141,47 @@ Proof.
           destruct Hlookup_p as [(<- & <-) | (Hkey_p_neq & Hlookup_p)];
           destruct Hlookup_c as [(<- & <-) | (Hkey_c_neq & Hlookup_c)].
           + exfalso. by apply (Hno_self_parenting key s key Hlookup_children Hkey_in_s).
-          + rewrite updated_pure_pod_uid_eq. eapply Hchildren_point_to_parent; [done|done|done|done].
-          + unfold obj_has_controller_parent_of. rewrite updated_pure_pod_owner_references_eq.
+          + rewrite updated_pure_kobj_uid_eq. eapply Hchildren_point_to_parent; [done|done|done|done].
+          + unfold obj_has_controller_parent_of. rewrite updated_pure_kobj_owner_references_eq.
             eapply Hchildren_point_to_parent; [done|done|done|done].
           + eapply Hchildren_point_to_parent; [done|done|done|done].
-          + rewrite updated_pure_pod_uid_eq in Hobj_has_controller_parent_of.
-            pose proof ((proj2 (Hchildren_point_to_parent _ _ _ _ _ Hkey_in_abs Hkey_in_abs Hlookup_children) Hobj_has_controller_parent_of)). done.
-          + rewrite updated_pure_pod_uid_eq in Hobj_has_controller_parent_of.
+          + assert (obj_has_controller_parent_of pure_kobj (KKey.Kind' key) (KKey.Name' key)
+              (PureObjectMeta.UID' (PureKObject.objectmeta pure_kobj))) as H.
+            { rewrite updated_pure_kobj_uid_eq in Hobj_has_controller_parent_of. destruct pure_kobj; done. }
+            pose proof ((proj2 (Hchildren_point_to_parent _ _ _ _ _ Hkey_in_abs Hkey_in_abs Hlookup_children) H)). done.
+          + rewrite updated_pure_kobj_uid_eq in Hobj_has_controller_parent_of.
             pose proof ((proj2 (Hchildren_point_to_parent _ _ _ _ _ Hkey_in_abs Hlookup_c Hlookup_children) Hobj_has_controller_parent_of)). done.
           + unfold obj_has_controller_parent_of in Hobj_has_controller_parent_of.
-            rewrite updated_pure_pod_owner_references_eq in Hobj_has_controller_parent_of.
+            rewrite updated_pure_kobj_owner_references_eq in Hobj_has_controller_parent_of.
             pose proof ((proj2 (Hchildren_point_to_parent _ _ _ _ _ Hlookup_p Hkey_in_abs Hlookup_children) Hobj_has_controller_parent_of)). done.
           + pose proof ((proj2 (Hchildren_point_to_parent _ _ _ _ _ Hlookup_p Hlookup_c Hlookup_children) Hobj_has_controller_parent_of)). done.
-        - intros k obj kind name uid Hlookup Href.
+        - intros k o kind name uid Hlookup Href.
           rewrite lookup_insert_Some in Hlookup.
           destruct Hlookup as [(<- & <-) | (Hkey_neq & Hlookup)].
           + unfold obj_has_controller_parent_of in Href.
-            rewrite updated_pure_pod_owner_references_eq in Href.
+            rewrite updated_pure_kobj_owner_references_eq in Href.
             eapply Hparent_uid_is_used; [done|done].
           + eapply Hparent_uid_is_used; [done|done].
       }
       iCombineNamed "Hinv_*" as "H".
       wp_apply (wp_Mutex__Unlock _ (kubernetes_inv γ l) with "[$Hown_Mutex H]").
       { iNamed "H". iFrame. iFrame "#". done. }
-      iApply "HΦ". iLeft. iFrame. done.
-    + iDestruct (struct_fields_combine (V:=v1.Pod.t) with "[$HTypeMeta $HObjectMeta $HSpec $HStatus]") as "Hpod_ptr".
-      iAssert (⌜ pure_pod.(PurePod.ObjectMeta').(PureObjectMeta.DeletionTimestamp') ≠ None ⌝%I) as "%Hdeletiontimestamp_not_none". {
-        iNamed "Hdeepown_pod". iNamed "Hdeepown_objectmeta". iPureIntro. intros H. apply (proj2 Hdeepown_deletiontimestamp_none) in H. done. }
-      iAssert (state_rep phys_state abs_state %I) with "[Hpod_ptr Hother_rep Hdeepown_pod]" as "Hinv_Hphys_abs_rep". {
-        iApply big_sepM2_delete; [done | done|]. iFrame. unfold obj_rep. rewrite kind_is_pod.
-        iExists ptr, pod, pure_pod. iFrame. iFrame "#". done. }
+      iApply "HΦ". iLeft. iFrame. iPureIntro. destruct pure_kobj; done.
+    + iAssert (⌜ (PureKObject.objectmeta pure_kobj).(PureObjectMeta.DeletionTimestamp') ≠ None ⌝%I) as "%Hdt".
+      { iNamed "Hdeepown_objectmeta". iPureIntro. intros H. apply (proj2 Hdeepown_deletiontimestamp_none) in H. done. }
+      iPoseProof (PureKObject.deepown_l_restore _ _ _ _
+        with "[Htypemeta_ptr Hobjectmeta_ptr Hdeepown_objectmeta Hdeepown_l_other]") as "Hdeepown_l".
+      { iFrame. done. }
+      iAssert (PureKObject.deepown_l ptr kobj pure_kobj 1) with "[Hdeepown_l]" as "Hdeepown_l".
+      { destruct pure_kobj; iFrame. }
+      iAssert (state_rep phys_state abs_state %I) with "[Hdeepown_l Hother_rep]" as "Hinv_Hphys_abs_rep".
+      { iApply big_sepM2_delete; [done | done|]. iFrame. iPureIntro. destruct pure_kobj; done. }
       iCombineNamed "Hinv_*" as "H".
       wp_apply (wp_Mutex__Unlock _ (kubernetes_inv γ l) with "[$Hown_Mutex H]").
       { iNamed "H". iFrame. iFrame "#". done. }
-      iApply "HΦ". iLeft. iFrame. done.
+      iApply "HΦ". iLeft. iFrame. destruct pure_kobj; done.
   - wp_apply (wp_map_delete with "[$Hinv_Hown_phys]"). iIntros "Hinv_Hown_phys". wp_auto.
-    iDestruct (struct_fields_combine (V:=v1.Pod.t)
-      with "[$HTypeMeta $HObjectMeta $HSpec $HStatus]") as "Hpod_ptr".
-    iMod (auth_map.map_delete with "Hown_pod Hinv_Hown_abs") as "Hinv_Hown_abs".
+    iMod (auth_map.map_delete with "Hghost_pure_kobj Hinv_Hown_abs") as "Hinv_Hown_abs".
     iMod (auth_map.map_update _ _ (owned_child_keys ∖ {[key]}) with "Hinv_Hown_children Hown_child_keys")
       as "[Hinv_Hown_children Hown_child_keys]".
     iMod (auth_map.map_delete with "Hown_grandchild_keys Hinv_Hown_children") as "Hinv_Hown_children".
@@ -195,7 +190,7 @@ Proof.
     {
       destruct Hinv_Hghost_well_formed.
       assert (parent_key ≠ key) as parent_neq_key.
-      { specialize (Hno_self_parenting parent_key owned_child_keys key Hparent_key_in_children Hpod_is_child). done. }
+      { specialize (Hno_self_parenting parent_key owned_child_keys key Hparent_key_in_children His_child). done. }
       assert (dom (delete key (<[parent_key:=owned_child_keys ∖ {[key]}]> children)) = dom (delete key children) )
       as Hdom_children_eq. {
         assert (key ≠ parent_key) as key_neq_parent by (symmetry; exact parent_neq_key).
@@ -206,7 +201,7 @@ Proof.
         { set_solver. }
         reflexivity. }
       apply mk_ghost_well_formed.
-      - intros k obj Hlookup. rewrite lookup_delete_Some in Hlookup.
+      - intros k o Hlookup. rewrite lookup_delete_Some in Hlookup.
         eapply Habs_state_well_formed. intuition.
       - set_solver.
       - intros k s Hlookup.
@@ -221,7 +216,7 @@ Proof.
           assert (s ## owned_child_keys) as s_disj_owned.
           { destruct (decide (k = parent_key)); [congruence|]. eapply Hchildren_disjoint; done. }
           assert (key ∉ s) as key_not_in_s.
-          { intros Hcontra. assert (key ∈ owned_child_keys) by exact Hpod_is_child. set_solver. }
+          { intros Hcontra. assert (key ∈ owned_child_keys) by exact His_child. set_solver. }
           set_solver.
       - intros k s child_key Hlookup Hchild_in_s.
         rewrite lookup_delete_Some lookup_insert_Some in Hlookup.
@@ -257,7 +252,7 @@ Proof.
         destruct Hlookup1 as (Hk1_neq_key & Hlookup_obj1).
         destruct Hlookup2 as (Hk2_neq_key & Hlookup_obj2).
         eapply Hno_duplicate_uid; [eauto|eauto|done].
-      - intros k obj Hlookup.
+      - intros k o Hlookup.
         rewrite lookup_delete_Some in Hlookup.
         destruct Hlookup as (Hk_neq_key & Hlookup_obj).
         eapply Hexisting_uid_is_used. done.
@@ -277,7 +272,7 @@ Proof.
           pose proof ((proj2 (Hchildren_point_to_parent _ _ _ _ _ Hlookup_p Hlookup_c Hparent_key_in_children) Hobj_has_controller_parent_of)). set_solver.
         + intros Hobj_has_controller_parent_of.
           pose proof ((proj2 (Hchildren_point_to_parent _ _ _ _ _ Hlookup_p Hlookup_c Hlookup_children) Hobj_has_controller_parent_of)). done.
-      - intros k obj kind name uid Hlookup.
+      - intros k o kind name uid Hlookup.
         rewrite lookup_delete_Some in Hlookup.
         destruct Hlookup as (Hk_neq_key & Hlookup_obj).
         eapply Hparent_uid_is_used. done.
@@ -294,16 +289,15 @@ Lemma wp_State__PodDelete γ l namespace name
   {{{ is_pkg_init apimodel ∗
       "#inv" ∷ is_kubernetes γ l ∗
       "%Hkey_eq" ∷ ⌜ key = mk_pod_key namespace name ⌝ ∗
-      "Hown_pod" ∷ key [[ γ.(γ_state) ]]↦ (PureKObject.Pod pure_pod) ∗
+      "Hghost_pure_pod" ∷ key [[ γ.(γ_state) ]]↦ (PureKObject.Pod pure_pod) ∗
       "Hown_child_keys" ∷ parent_key [[ γ.(γ_children) ]]↦ owned_child_keys ∗
       "Hown_grandchild_keys" ∷ key [[ γ.(γ_children) ]]↦ owned_grandchild_keys ∗
-      "%Hpod_is_child" ∷ ⌜ key ∈ owned_child_keys ⌝
+      "%His_child" ∷ ⌜ key ∈ owned_child_keys ⌝
   }}}
     l @ (ptrT.id apimodel.State.id) @ "PodDelete" #namespace #name
-  {{{ updated_pure_pod, RET #interface.nil;
-      "Hpod_updated_or_deleted" ∷ ((
-        "%Hts" ∷ ⌜ updated_pure_pod.(PurePod.ObjectMeta').(PureObjectMeta.DeletionTimestamp') ≠ None ⌝ ∗
-        "Hown_pod" ∷ key [[ γ.(γ_state) ]]↦ (PureKObject.Pod updated_pure_pod) ∗
+  {{{ pure_pod', RET #interface.nil;
+      (("%Hts" ∷ ⌜ pure_pod'.(PurePod.ObjectMeta').(PureObjectMeta.DeletionTimestamp') ≠ None ⌝ ∗
+        "Hghost_pure_pod" ∷ key [[ γ.(γ_state) ]]↦ (PureKObject.Pod pure_pod') ∗
         "Hown_child_keys" ∷ parent_key [[ γ.(γ_children) ]]↦ owned_child_keys ∗
         "Hown_grandchild_keys" ∷ key [[ γ.(γ_children) ]]↦ owned_grandchild_keys
       ) ∨
@@ -311,9 +305,15 @@ Lemma wp_State__PodDelete γ l namespace name
   }}}.
 Proof.
   wp_start as "H". iNamed "H". subst key. wp_auto.
-  wp_apply (wp_State__objDelete_pod with "[$Hown_pod $Hown_child_keys $Hown_grandchild_keys]").
+  wp_apply (wp_State__objDelete with "[$Hghost_pure_pod $Hown_child_keys $Hown_grandchild_keys]").
   { iFrame "#". done. }
-  iIntros (updated_pure_pod) "H". iNamed "H". wp_auto. iApply "HΦ". iFrame.
+  iIntros (pure_kobj') "H". wp_auto. iDestruct "H" as "[H|H]".
+  - iNamed "H".
+    assert (∃ pure_pod', pure_kobj' = PureKObject.Pod pure_pod') as [pure_pod' ->].
+    { destruct pure_kobj'; try done. exists p. done. }
+    iApply "HΦ". iLeft. iFrame. done.
+  - iApply "HΦ". iRight. iFrame. 
+  Unshelve. done.
 Qed.
 
 End proof.
