src/proof/get.v
@@ -8,58 +8,55 @@ Context `{!mapG Σ KKey.t PureKObject.t}.
 Context `{!mapG Σ KKey.t (gset KKey.t)}.
 Context `{!auth_setG Σ KKey.t}.
 
-Lemma wp_State__objGet_replicaset γ l key pure_rs:
+Lemma wp_State__objGet γ l key pure_kobj:
   {{{ is_pkg_init apimodel ∗
       "#Hisk" ∷ is_kubernetes γ l ∗
-      "%Hkind_eq" ∷ ⌜ KKey.Kind' key = "ReplicaSet"%go ⌝ ∗
-      "Hown_rs" ∷ key [[ γ.(γ_state) ]]↦ (PureKObject.ReplicaSet pure_rs)
+      "%Hkind_eq" ∷ ⌜ KKey.Kind' key = PureKObject.kind pure_kobj ⌝ ∗
+      "Hghost" ∷ key [[ γ.(γ_state) ]]↦ pure_kobj
   }}}
     l @ (ptrT.id apimodel.State.id) @ "objGet" #key
-  {{{ ptr rs, RET (#(interface.mk (ptrT.id v1.ReplicaSet.id) #ptr), #true);
-      PureReplicaSet.deepown_l ptr rs pure_rs 1 ∗
-      ⌜ PureReplicaSet.well_formed pure_rs ⌝ ∗
-      ⌜ key.(KKey.Namespace') = pure_rs.(PureReplicaSet.ObjectMeta').(PureObjectMeta.Namespace') ⌝ ∗
-      ⌜ key.(KKey.Name') = pure_rs.(PureReplicaSet.ObjectMeta').(PureObjectMeta.Name') ⌝ ∗
-      key [[ γ.(γ_state) ]]↦ (PureKObject.ReplicaSet pure_rs)
+  {{{ obj ptr kobj, RET (#obj, #true);
+      ⌜ PureKObject.interface_agree obj ptr pure_kobj ⌝ ∗
+      PureKObject.deepown_l ptr kobj pure_kobj 1 ∗
+      ⌜ PureKObject.well_formed pure_kobj ⌝ ∗
+      ⌜ key.(KKey.Namespace') = (PureKObject.objectmeta pure_kobj).(PureObjectMeta.Namespace') ⌝ ∗
+      ⌜ key.(KKey.Name') = (PureKObject.objectmeta pure_kobj).(PureObjectMeta.Name') ⌝ ∗
+      key [[ γ.(γ_state) ]]↦ pure_kobj
   }}}.
 Proof.
   wp_start as "H". iNamed "H". iNamed "Hisk".
   wp_apply wp_with_defer. iIntros (defer) "Hdefer". simpl subst. wp_auto.
   wp_apply wp_Mutex__Lock; [done|]. iIntros "[Hown_Mutex H]". iNamedPrefix "H" "Hinv_". wp_auto.
-  iAssert (⌜ abs_state !! key = Some (PureKObject.ReplicaSet pure_rs) ⌝%I) with "[Hown_rs Hinv_Hown_abs]" as "%Hkey_in_abs".
-  { iDestruct (map_valid with "Hinv_Hown_abs Hown_rs") as %Hlookup.
+  iAssert (⌜ abs_state !! key = Some pure_kobj ⌝%I) with "[Hghost Hinv_Hown_abs]" as "%Hkey_in_abs".
+  { iDestruct (map_valid with "Hinv_Hown_abs Hghost") as %Hlookup.
     iPureIntro; exact Hlookup. }
   iAssert (⌜ ∃ obj, phys_state !! key = Some obj ⌝%I) with "[Hinv_Hphys_abs_rep]" as "%Hinv_Hkey_in_phys".
   { iDestruct (big_sepM2_lookup_r with "Hinv_Hphys_abs_rep") as (obj Hkey_in_phys) "_".
     { exact Hkey_in_abs. }
     iPureIntro. exists obj. exact Hkey_in_phys. }
   destruct Hinv_Hkey_in_phys as [obj Hinv_Hkey_in_phys].
-  iDestruct (big_sepM2_lookup_acc _ _ _ _ _ _ Hinv_Hkey_in_phys Hkey_in_abs with "Hinv_Hphys_abs_rep") as "[Hk_rep Hother_rep]".
-  destruct decide_kind_is_replicaset with (KKey.Kind' key) as [Hkind_is_replicaset Hkind_is_not_pod]; [done|].
-  unfold obj_rep. rewrite Hkind_is_replicaset Hkind_is_not_pod.
-  iDestruct "Hk_rep" as "(%ptr & %rs & %pure_rs' & H)". iNamed "H". injection Habs_v_is_rs as <-.
+  iDestruct (big_sepM2_lookup_acc _ _ _ _ _ _ Hinv_Hkey_in_phys Hkey_in_abs with "Hinv_Hphys_abs_rep")
+    as "(Hk_rep & Hother_rep)".
+  iDestruct "Hk_rep" as "(%ptr & %kobj & %Hinterface_agree & Hdeepown_l)".
   wp_apply (wp_map_get with "[$Hinv_Hown_phys]"). iIntros "Hinv_Hown_phys". wp_auto.
   rewrite /is_Some Hinv_Hkey_in_phys. wp_auto.
-  wp_apply (wp_deepCopy_replicaset with "[$Hdeepown_l_rs]"); [done|].
-  iIntros (copied_ptr copied_rs) "(Hdeepown_l_copied_rs & Hdeepown_l_rs)". wp_auto.
-  iAssert (state_rep phys_state abs_state) with "[Hdeepown_l_rs Hother_rep]" as "Hinv_Hphys_abs_rep".
-  { iApply "Hother_rep". iExists ptr, rs, pure_rs. iFrame. done. }
-  assert (key = PureKObject.key (PureKObject.ReplicaSet pure_rs) ∧ PureKObject.well_formed (PureKObject.ReplicaSet pure_rs))
-    as [Hkey_eq Hwell_formed].
+  wp_apply (wp_deepCopy with "[$Hdeepown_l]"); [done|].
+  iIntros (obj' ptr' kobj') "(%Hinterface_agree' & Hdeepown_l' & Hdeepown_l)". wp_auto.
+  iAssert (state_rep phys_state abs_state) with "[Hdeepown_l Hother_rep]" as "Hinv_Hphys_abs_rep".
+  { iApply "Hother_rep". iExists ptr, kobj. iFrame. done. }
+  assert (key = PureKObject.key pure_kobj ∧ PureKObject.well_formed pure_kobj) as [-> Hwell_formed].
   { destruct Hinv_Hghost_well_formed. apply Habs_state_well_formed. exact Hkey_in_abs. }
   iCombineNamed "Hinv_*" as "H".
-  wp_apply (wp_Mutex__Unlock _ (kubernetes_inv γ l)
-  with "[$Hown_Mutex H]").
+  wp_apply (wp_Mutex__Unlock _ (kubernetes_inv γ l) with "[$Hown_Mutex H]").
   { iNamed "H". iFrame. iFrame "#". done. }
-  iApply "HΦ". iFrame. iPureIntro. split; [done|].
-  unfold PureKObject.key in Hkey_eq. unfold PureReplicaSet.key in Hkey_eq. rewrite Hkey_eq. done.
+  iApply "HΦ". iFrame. iPureIntro. split; [done|]. split_and!;[done|done|done].
 Qed.
 
 Lemma wp_State__ReplicaSetMutGet γ l key namespace name pure_rs:
   {{{ is_pkg_init apimodel ∗
       "#Hisk" ∷ is_kubernetes γ l ∗
       "%Hkey_eq" ∷ ⌜ key = (mk_replicaset_key namespace name) ⌝ ∗
-      "Hown_rs" ∷ key [[ γ.(γ_state) ]]↦ (PureKObject.ReplicaSet pure_rs)
+      "Hghost" ∷ key [[ γ.(γ_state) ]]↦ (PureKObject.ReplicaSet pure_rs)
   }}}
     l @ (ptrT.id apimodel.State.id) @ "ReplicaSetMutGet" #namespace #name
   {{{ ptr rs, RET (#ptr, #interface.nil);
@@ -71,8 +68,9 @@ Lemma wp_State__ReplicaSetMutGet γ l key namespace name pure_rs:
   }}}.
 Proof.
   wp_start as "H". iNamed "H". wp_auto. subst key. unfold mk_replicaset_key.
-  wp_apply (wp_State__objGet_replicaset with "[$Hown_rs]"); [iFrame "#";done|].
-  iIntros (ptr rs) "(Hdeepown_l_rs & %Hwell_formed_pure_rs & <- & <- & Hown_pure_rs)". wp_auto.
+  wp_apply (wp_State__objGet with "[$Hghost]"); [iFrame "#";done|].
+  iIntros (obj ptr kobj) "(%Hinterface_agree & Hdeepown_l & %Hwf & %Hns_eq & %Hname_eq & Hghost)". wp_auto.
+  unfold PureKObject.interface_agree in Hinterface_agree. rewrite Hinterface_agree.
   unshelve wp_apply wp_interface_checked_type_assert; try tc_solve.
   { iPureIntro. intros ptr_id. exists ptr. done. }
   iIntros (y ok) "%if_ok".
@@ -81,6 +79,7 @@ Proof.
   wp_auto.
   assert (ptr = y) as ->.
   { inversion if_ok. apply (inj to_val). done. }
+  iPoseProof (PureKObject.replicaset_deepown_l with "Hdeepown_l") as "(%rs & -> & Hdeepown_l)".
   iApply "HΦ". iFrame. done.
 Qed.
 
@@ -88,7 +87,7 @@ Lemma wp_State__ReplicaSetGet γ l key namespace name pure_rs:
   {{{ is_pkg_init apimodel ∗
       "#Hisk" ∷ is_kubernetes γ l ∗
       "%Hkey_eq" ∷ ⌜ key = (mk_replicaset_key namespace name) ⌝ ∗
-      "Hown_rs" ∷ key [[ γ.(γ_state) ]]↦ (PureKObject.ReplicaSet pure_rs)
+      "Hghost" ∷ key [[ γ.(γ_state) ]]↦ (PureKObject.ReplicaSet pure_rs)
   }}}
     l @ (ptrT.id apimodel.State.id) @ "ReplicaSetGet" #namespace #name
   {{{ ptr rs dq, RET (#ptr, #interface.nil);
@@ -100,8 +99,8 @@ Lemma wp_State__ReplicaSetGet γ l key namespace name pure_rs:
   }}}.
 Proof.
   wp_start as "H". iNamed "H". wp_auto.
-  wp_apply (wp_State__ReplicaSetMutGet with "[$Hown_rs]"); [iFrame "#";done|].
-  iIntros (ptr rs) "(Hdeepown_l_rs & %Hwell_formed_pure_rs & <- & <- & Hown_rs)". wp_auto.
+  wp_apply (wp_State__ReplicaSetMutGet with "[$Hghost]"); [iFrame "#";done|].
+  iIntros (ptr rs) "(Hdeepown_l & %Hwf & <- & <- & Hghost)". wp_auto.
   iApply "HΦ". iFrame. done.
 Qed.
 
